

Fixed Income Derivatives E2025 - Problem Set Week 4

Problem 1

Let W_t be a Brownian motion, assume $s < t < u < v$ and solve the problems below. In doing so, you will need to use that W_t is Markov and has stationary independent increments. That is, for $0 < s < t$ we know that $W_t - W_s | \mathcal{F}_s = W_t - W_s | W_s = w_s \sim N(0, t - s)$.

- a) Find the conditional distribution of W_t given \mathcal{F}_s .
- c) Find $\mathbb{E}[W_s W_t]$, $\text{Cov}[W_s, W_t]$ and $\text{Cor}[X_t, Z_t]$.
- c) Show that $W_t^2 - t$ is a Martingale.
- d) Find $\mathbb{E}[W_s W_t W_u]$.
- e) Find $\mathbb{E}[W_s W_t W_u W_v]$.

Problem 1 - Solution

- a) $(W_t | W_s = w_s) \sim N(w_s, t - s)$.
- b) We of course have that $\text{Var}[W_s] = s$ and $\text{Var}[W_t] = t$ but also

$$\begin{aligned}\mathbb{E}[W_s W_t] &= \mathbb{E}[\mathbb{E}[W_s W_t | \mathcal{F}_s]] = \mathbb{E}[\mathbb{E}[W_s W_t | \mathcal{F}_s]] = \mathbb{E}[W_s^2] = s \\ \text{Cov}[W_s, W_t] &= \mathbb{E}[W_s W_t] - \mathbb{E}[W_s] \mathbb{E}[W_t] = s \\ \text{Cor}[X_t, Z_t] &= \frac{s}{\sqrt{s} \sqrt{t}} = \sqrt{\frac{s}{t}}\end{aligned}\tag{1}$$

- c) To show that $W_t^2 - t$ is a Martingale, we need to show that $\mathbb{E}[W_t^2 - t | \mathcal{F}_s] = W_s^2 - s$.

$$\begin{aligned}\mathbb{E}[W_t^2 - t | \mathcal{F}_s] &= \mathbb{E}[(W_t - W_s + W_s)^2 - t | \mathcal{F}_s] = \mathbb{E}[(W_t - W_s)^2 + 2(W_t - W_s)W_s + W_s^2 - t | \mathcal{F}_s] \\ &= \mathbb{E}[(W_t - W_s)^2 + 2W_t W_s - W_s^2 - t | \mathcal{F}_s] = (t - s) + 2W_s^2 - W_s^2 - t = W_s^2 - s\end{aligned}\tag{2}$$

- d) Let us find $\mathbb{E}[W_s W_t W_u]$ by conditioning

$$\begin{aligned}\mathbb{E}[W_s W_t W_u] &= \mathbb{E}[\mathbb{E}[W_s W_t W_u | \mathcal{F}_t]] = \mathbb{E}[W_s W_t \mathbb{E}[W_u | \mathcal{F}_t]] = \mathbb{E}[W_s W_t^2] \\ &= \mathbb{E}[\mathbb{E}[W_s W_t^2 | \mathcal{F}_s]] = \mathbb{E}[W_s \mathbb{E}[W_t^2 | \mathcal{F}_s]] = \mathbb{E}[W_s(t - s + W_s^2)] = (t - s)\mathbb{E}[W_s] + \mathbb{E}[W_s^3] = 0\end{aligned}$$

- e) Let us find $\mathbb{E}[W_s W_t W_u W_v]$ once again by conditioning

$$\begin{aligned}\mathbb{E}[W_s W_t W_u W_v] &= \mathbb{E}[\mathbb{E}[W_s W_t W_u W_v | \mathcal{F}_u]] = \mathbb{E}[W_s W_t W_u \mathbb{E}[W_v | \mathcal{F}_u]] = \mathbb{E}[W_s W_t W_u^2] \\ &= \mathbb{E}[W_s W_t \mathbb{E}[W_u^2 | \mathcal{F}_t]] = \mathbb{E}[W_s W_t(u - t + W_t^2)] = s(u - t) + \mathbb{E}[W_s \mathbb{E}[W_t^3 | \mathcal{F}_s]] \\ &= s(u - t) + \mathbb{E}[W_s(W_s^3 + 3W_s(t - s))] = s(u - t) + 3s^2 + 3s(t - s) = s(2t + u)\end{aligned}\tag{3}$$

Problem 2

Let X_t and Y_t be independent Brownian motions for $t \geq 0$. Define $Z_t = \rho X_t + \sqrt{1 - \rho^2} Y_t$.

- a) Show that Z_t is a Brownian motion
- b) Find $\text{Cor}[X_t, Z_t]$.
- c) Find $\mathbb{E}[Z_t | X_t = x]$ and $\text{Var}[Z_t | X_t = x]$.

Let $W_t^{(1)}, W_t^{(2)}, \dots, W_t^{(N)}$ be independent Brownian motions and let Σ be an $M \times N$ -dimensional matrix where row i , Σ_i , satisfies $\|\Sigma_i\| = \Sigma_{i1}^2 + \Sigma_{i2}^2 + \dots + \Sigma_{iN}^2 = 1$. Define the M -dimensional vector $\mathbf{Y}_t = \Sigma \mathbf{W}_t$

- d) Find the covariance matrix of the random vector \mathbf{Y}_t . Show that the covariance matrix is positive definite?

- e) What is the correlation matrix of \mathbf{Y}_t ?
- f) What is the distribution of $Y_t^{(i)}$ and what is the joint distribution of \mathbf{Y}_t ?
- g) Is \mathbf{Y}_t a multivariate Brownian motion?

Problem 2 - Solution

- a) X_t and Y_t have stationary independent increments and therefore, Z_t has stationary independent increments. $Z_t - Z_s$ is the sum of two independent Gaussian random variables and is also Gaussian.

$$\begin{aligned}\mathbb{E}[Z_t - Z_s | \mathcal{F}_s] &= \rho \mathbb{E}[X_t - X_s | \mathcal{F}_s] + \sqrt{1 - \rho^2} \mathbb{E}[Y_t - Y_s | \mathcal{F}_s] = \rho \cdot 0 + \sqrt{1 - \rho^2} \cdot 0 \\ \text{Var}[Z_t - Z_s | \mathcal{F}_s] &= \mathbb{E}[(Z_t - Z_s)^2 | \mathcal{F}_s] = \rho^2 \mathbb{E}[(X_t - X_s)^2 | \mathcal{F}_s] + (1 - \rho^2) \mathbb{E}[(Y_t - Y_s)^2 | \mathcal{F}_s] \\ &= \rho^2(t - s) + (1 - \rho^2)^2(t - s) = t - s\end{aligned}\quad (4)$$

In conclusion, Z_t is a continuous stochastic process that has stationary independent increments each of which are Gaussian with mean 0 and variance proportional to time. Thus, Z_t is a Brownian motion.

- b) We note that $\mathbb{E}[X_t] = 0$, $\mathbb{E}[Z_t] = 0$, $\text{Var}[X_t] = t$ and $\text{Var}[Z_t] = t$

$$\begin{aligned}\text{Cov}[Z_t X_t] &= \mathbb{E}[Z_t X_t] = \mathbb{E}[(\rho X_t + \sqrt{1 - \rho^2} Y_t) X_t] = \rho \mathbb{E}[X_t^2] + \sqrt{1 - \rho^2} \mathbb{E}[X_t Y_t] = \rho t \\ \text{Cor}[Z_t X_t] &= \frac{\text{Cov}[Z_t X_t]}{\sqrt{\text{Var}[X_t]} \sqrt{\text{Var}[Z_t]}} = \rho\end{aligned}\quad (5)$$

- c) The conditional mean and variance of Z_t given $X_t = x$ can be found from

$$\begin{aligned}\mathbb{E}[Z_t | X_t = x] &= \mathbb{E}[\rho X_t | X_t = x] + \sqrt{1 - \rho^2} \mathbb{E}[Y_t | X_t = x] = \rho x \\ \text{Var}[Z_t | X_t = x] &= \mathbb{E}[(\rho X_t + \sqrt{1 - \rho^2} Y_t - \rho x)^2 | X_t = x] \\ &= \mathbb{E}[(\rho X_t - \rho x)^2 | X_t = x] + 2\mathbb{E}[(\rho X_t - \rho x) | X_t = x] \mathbb{E}[\sqrt{1 - \rho^2} Y_t | X_t = x] + (1 - \rho^2) \mathbb{E}[Y_t^2 | X_t = x] \\ &= (1 - \rho^2)t\end{aligned}\quad (6)$$

- d) Let us find the moments of the vector \mathbf{Y}_t . Denote dot product by \cdot , use Y_i for the i th entry of \mathbf{Y}_t , use Σ_{ij} for the entry in the i th row and j th column of Σ and finally use $\Sigma_{i\cdot}$ to denote the i 'th row of Σ . Then

$$\begin{aligned}\mathbb{E}[Y_i] &= \mathbb{E}\left[\sum_{n=1}^N \Sigma_{in} W_t^{(n)}\right] = 0 \\ \text{Var}[Y_i] &= \mathbb{E}[Y_i^2] = \mathbb{E}\left[\sum_{m=1}^M \sum_{n=1}^N \Sigma_{im} \Sigma_{in} W_t^{(m)} W_t^{(n)}\right] = t \sum_{n=1}^N \Sigma_{in}^2 = t \Sigma_{i\cdot} \cdot \Sigma_{i\cdot} = t \|\Sigma_{i\cdot}\|^2 = t \\ \text{Cov}[Y_i Y_j] &= \mathbb{E}[Y_i Y_j] = \mathbb{E}\left[\sum_{m=1}^M \sum_{n=1}^N \Sigma_{im} \Sigma_{jn} W_t^{(m)} W_t^{(n)}\right] = t \sum_{n=1}^N \Sigma_{in} \Sigma_{jn} = t \Sigma_{i\cdot} \cdot \Sigma_{j\cdot}\end{aligned}\quad (7)$$

The covariance matrix of \mathbf{Y}_t can therefore be written as

$$\text{Cov}[\mathbf{Y}_t] = \text{Cov}[\Sigma \mathbf{W}_t] = \Sigma \Sigma', \quad \Omega = \begin{bmatrix} t & 0 & \cdots & 0 \\ 0 & t & \cdots & 0 \\ \vdots & \vdots & \ddots & \vdots \\ 0 & 0 & \cdots & t \end{bmatrix}\quad (8)$$

This matrix is positive definite by construction since, we can write $\text{Cov}[\mathbf{Y}_t]$ as the matrix square of two matrices

$$\text{Cov}[\mathbf{Y}_t] = \Sigma \Sigma' = \mathbf{A} \mathbf{A}'\quad (9)$$

e) The correlation between Y_i and Y_j is thus $\text{Cor}[Y_i Y_j] = \Sigma_i \Sigma_j$. and the correlation matrix of \mathbf{Y}_t is

$$\text{Cor}[\mathbf{Y}_t] = \text{Cor}[\Sigma \mathbf{W}_t] = \Sigma \Sigma' \quad (10)$$

f) $Y_t^{(i)}$ is the sum of independent Gaussian random variables and is itself Gaussian with mean 0 and variance t for all t . Furthermore, $Y_t^{(i)}$ has continuous trajectories and hence, $Y_t^{(i)}$ is a Brownian motion. Now since $Y_t^{(i)}$ is a sum of independent normal random variables for all i , it follows that any linear combination $\mathbf{b}' \mathbf{Y}_t$, $\mathbf{b} \in \mathbb{R}^n$ is also a Gaussian random variable. Hence, the joint distribution of the processes collected in $\mathbf{Y}_t^{(i)}$ is multivariate normal

$$\mathbf{Y}_t \sim N(\mathbf{0}, \Sigma \Omega \Sigma'). \quad (11)$$

g) We can therefore define \mathbf{Y}_t as a multivariate Brownian motion with correlation matrix $\Sigma \Sigma'$ and we have just seen a very straight-forward method to construct a multivariate Brownian motion with a specific correlation matrix.

Problem 3

Consider a stochastic process r_t for $t \geq 0$ with dynamics

$$dr_t = (b - ar_t)dt + \sigma dW_t, \quad b > 0$$

a) Show that the solution $r(T)$ corresponding to these dynamics are

$$r_T = e^{-aT} r_0 + \frac{b}{a} (1 - e^{-aT}) + \sigma \int_0^T e^{-a(T-t)} dW_t$$

by performing the following steps

- i) Apply Ito's formula to $f(t, r) = e^{at} r$.
- ii) Simplify to get an expression for $d(e^{at} r)$ that does not depend on r_t .
- iii) Integrate from 0 to T and solve the time-integral.
- b) Use Ito isometry to show that $r_T | r_t \sim N\left(e^{-aT} r_0 + \frac{b}{a} (1 - e^{-aT}), \frac{\sigma^2}{2a} [1 - e^{-2aT}]\right)$.
- c) Find the limiting distribution of r_T as $T \nearrow \infty$.
- d) If you had to guess, what is your best guess of the r in the long run? How does the limiting distribution of r_T depend on r_0 and what is the implication?

Problem 3 - Solution

a) The SDE in (12) can be solved explicitly by applying *Ito* to $f(t, r_t) = e^{at} r_t$

$$df(t, r_t) = ae^{at} r_t dt + e^{at} (b - ar_t) dt + e^{at} dW_t = be^{at} dt + \sigma e^{at} dW_t \quad (12)$$

Integrating from t to T gives us that

$$\begin{aligned} \int_t^T df(u, r_u) &= e^{aT} r_T - e^{at} r_t = \int_t^T be^{au} du + \sigma \int_t^T e^{au} dW_u \Rightarrow \\ r_T &= r_t e^{-a(T-t)} + be^{-aT} \int_t^T e^{au} du + \sigma \int_t^T e^{-a(T-u)} dW_u \end{aligned}$$

and hence, the solution becomes

$$r_T = r_t e^{-a(T-t)} + \frac{b}{a} [1 - e^{-a(T-t)}] + \sigma \int_t^T e^{-a(T-u)} dW_u. \quad (13)$$

- b) We know that from Problem 5) below that an Ito integral with a deterministic integrand will follow a Gaussian distribution. We also know that the expected value of an Ito integral is 0, so we have

$$\mathbb{E}[r_T|r_t] = e^{-aT}r_0 + \frac{b}{a}(1 - e^{-aT}) \quad (14)$$

Computing the variance of $r_T|r_t$ gives us that

$$\text{Var}[r_T|r_t] = \mathbb{E}\left[\left(\sigma \int_t^T e^{-a(T-u)} dW_u\right)^2 | r_t\right] \stackrel{\text{Ito isometry}}{=} \sigma^2 \int_t^T e^{-2a(T-u)} du = \frac{\sigma^2}{2a}[1 - e^{-2aT}] \quad (15)$$

and we conclude that

$$r_T|r_t \sim N\left(e^{-aT}r_0 + \frac{b}{a}(1 - e^{-aT}), \frac{\sigma^2}{2a}[1 - e^{-2aT}]\right) \quad (16)$$

- c) Sending $T \nearrow \infty$ to find the limiting distribution gives us that

$$r_\infty \sim N\left(\frac{b}{a}, \frac{\sigma^2}{2a}\right) \quad (17)$$

The fact that the limiting distribution exists and is well-defined allows us to conclude that the short rate in this model settles to a stationary distribution.

- d) The long run mean under the stationary distribution is $\frac{b}{a}$ and that would be our best long-run guess for the short rate. The limiting distribution does not depend on r_0 implying that this process forgets its origin. The mean of $r_T|r_t$ for T finite is a weighted average of the initial value r_t and the long-run mean $\frac{b}{a}$ where the weight on r_t decays exponentially fast and at the rate a . Likewise, $\text{Var}[r_T|r_t]$ also decays exponentially fast at a rate of $2a$ to the long-run variance. It is therefore quite clear that the parameter a governs the rate at which the distribution of the short rate settles to its stationary distribution.

Problem 4

Suppose that the stochastic process S_t follows a Geometric Brownian motion and has dynamics

$$\begin{aligned} dS_t &= \mu S_t dt + \sigma S_t dW_t \\ S_0 &= s_0 \end{aligned}$$

- a) Show that the solution $S(T)$ corresponding to these dynamics is $S(T) = s_0 e^{(\mu - \frac{1}{2}\sigma^2)T + \sigma W_T}$.
b) Find $\mathbb{E}[S(T)]$ in terms of s_0 , μ and σ .
c) Find the dynamics of $Z_t = S_t^m$ and show that Z_t also follows a geometric Brownian motion.
d) Use these results to find $\mathbb{E}[S^m(T)]$.

Problem 4 - Solution

- a) Applying Ito to $X_t = \ln S_t$ and integrating from 0 to T will, as in Problem 2, give us that

$$S(T) = s_0 e^{(\mu - \frac{1}{2}\sigma^2)T + \sigma W_T} \quad (18)$$

- b) To find $\mathbb{E}[S(T)]$, we need to use that if

$$X \sim N(\mu, \sigma^2) \Rightarrow \mathbb{E}[e^{\omega X}] = e^{\omega\mu + \frac{1}{2}\omega^2\sigma^2} \quad (19)$$

We then get that

$$\mathbb{E}[S(T)] = s_0 e^{(\mu - \frac{1}{2}\sigma^2)T + \sigma W_T} = s_0 e^{(\mu - \frac{1}{2}\sigma^2)T} \mathbb{E}[e^{\sigma W(T)}] = s_0 e^{(\mu - \frac{1}{2}\sigma^2)T} e^{\frac{1}{2}\sigma^2 T} = s_0 e^{\mu T} \quad (20)$$

- c) We find the dynamics of $Z_t = S_t^m$ using Ito's formula

$$dZ_t = mS_t^{m-1}(\mu S_t dt + \sigma S_t dW_t) + \frac{1}{2}m(m-1)S_t^{m-2}\sigma^2 S_t^2 dt = (m\mu + \frac{1}{2}m(m-1)\sigma^2)Z_t dt + m\sigma Z_t dW_t \quad (21)$$

- d) From the dynamics of Z_t , we can see that Z_t follows a Geometric Brownian motion and hence

$$\mathbb{E}[S_t^m] = \mathbb{E}[Z_t] = e^{m\mu + \frac{1}{2}m(m-1)\sigma^2} \quad (22)$$

Problem 5

Let $\sigma(t)$ be a given *deterministic* function of time and define the process X_t by

$$X(t) = \int_0^t \sigma(s) dW_s$$

Also define $Z(t) = e^{i\omega X(t)}$ where i is the complex unit and thus a constant and ω is also a constant.

- Find the dynamics of X_t .
- Find the dynamics of Z_t and show that Z_t has dynamics

$$\begin{aligned} dZ_t &= -\frac{1}{2}\omega^2\sigma^2(t)Z(t)dt + i\omega\sigma(t)Z_t dW_t \\ Z_0 &= 1 \end{aligned}$$

- Integrate dZ_t and take expectations to find an expression for $\mathbb{E}[Z(t)]$.
- Define $m(t) = \mathbb{E}[Z(t)]$ and show that $m(t)$ satisfies the ODE.

$$\begin{aligned} m'(t) &= -\frac{1}{2}\omega^2\sigma^2(t)m(t) \\ m(0) &= 1 \end{aligned}$$

- Argue that $\mathbb{E}[e^{i\omega X(t)}] = \exp\left(-\frac{1}{2}\omega^2 \int_0^t \sigma^2(s)ds\right)$ and why we can say that $X(t) \sim N\left(0, \int_0^t \sigma^2(s)ds\right)$.

Problem 5 - Solution

- The dynamics of X_t can be found directly as $dX_t = \sigma_t dt$.
- Applying to $Z(t) = e^{i\omega X(t)}$ gives us that

$$dZ_t = d(e^{i\omega X(t)}) = i\omega e^{i\omega X(t)} dX_t - \frac{1}{2}\omega^2\sigma^2(t)e^{i\omega X(t)}(dX_t)^2 = -\frac{1}{2}\omega^2\sigma^2(t)Z(t)dt + i\omega\sigma(t)Z_t dW_t \quad (23)$$

- Integrating and taking expectations will now give us that

$$\begin{aligned} Z(t) &= Z(0) - \frac{1}{2}\omega^2 \int_0^t \sigma^2(s)Z(s)ds + i\omega \int_0^t \sigma(s)Z_s dW_s \Rightarrow \\ \mathbb{E}[Z(t)] &= 1 - \frac{1}{2}\omega^2 \int_0^t \sigma^2(s)\mathbb{E}[Z(s)]ds \end{aligned} \quad (24)$$

- Setting $m(t) = \mathbb{E}[Z(t)]$ we have directly from (24) that $m(t)$ satisfies the ODE

$$\begin{aligned} m'(t) &= -\frac{1}{2}\omega^2\sigma^2(t)m(t) \\ m(0) &= 1 \end{aligned} \quad (25)$$

- The solution to the ODE for $m(t)$ is

$$m(t) = \exp\left(-\frac{1}{2}\omega^2 \int_0^t \sigma^2(s)ds\right) \quad (26)$$

Now, we can put everything together to get that

$$\hat{f}_{X(t)}(\omega) = \mathbb{E}[e^{i\omega X(t)}] = \mathbb{E}[Z(t)] = \exp\left(-\frac{1}{2}\omega^2 \int_0^t \sigma^2(s)ds\right) \quad (27)$$

The function $\hat{f}_{X(t)}(\omega)$ is the characteristic function of a Gaussian random variable with mean 0 and variance $\int_0^t \sigma^2(s)ds$ and we conclude that

$$X(t) \sim N\left(0, \int_0^t \sigma^2(s)ds\right) \quad (28)$$